bf.v
@@ -10,6 +10,9 @@ Require Import Coq.Program.Tactics.
 Import ListNotations.
 
 Load parse.
+Load bftape.
+
+Print BFTape.
 
 Module BF.
 
@@ -152,25 +155,6 @@ Module BF.
   Qed.
 
   (* BF Interpreter *)
-  (* A BFTape is a map from [nat] indices to [Z] values *)
-  Module NatMap := FMapList.Make Nat_as_OT.
-  Definition BFTape := NatMap.t Z.
-
-  Definition tape_get (tape: BFTape) (ptr: nat): Z :=
-    match (NatMap.find ptr tape) with
-    | Some x => x
-    | None => 0
-    end.
-
-  Definition tape_set (tape: BFTape) (ptr: nat) (x: Z): BFTape :=
-    NatMap.add ptr x tape.
-
-  Definition tape_inc (tape: BFTape) (ptr: nat): BFTape :=
-    tape_set tape ptr (Z.succ (tape_get tape ptr)).
-
-  Definition tape_dec (tape: BFTape) (ptr: nat): BFTape :=
-    tape_set tape ptr (Z.pred (tape_get tape ptr)).
-
   (* `bf' is the current state of the program, while `resets' is the
      stack of programs to reset to at the end of a loop *)
   (* TODO: Generalize to all tape languages *)
@@ -178,14 +162,15 @@ Module BF.
     bf_state (bf: BF)
              (resets: list BF)
              (ptr: nat)
-             (tape: BFTape)
-             (input: list Z)
-             (output: list Z).
+             (tape: BFTape.Tape)
+             (input: list nat)
+             (output: list nat).
 
-  Function bf_state_init (bf: BF) (input: list Z): BFState :=
-    bf_state bf [] 0 (NatMap.empty Z) input [].
+  Print BFTape.
+  Function bf_state_init (bf: BF) (input: list nat): BFState :=
+    bf_state bf [] 0 BFTape.empty input [].
 
-  Function bf_state_output (state: BFState): list Z :=
+  Function bf_state_output (state: BFState): list nat :=
     match state with bf_state _ _ _ _ _ output => output end.
 
   Function bf_step (state: BFState): option BFState :=
@@ -203,20 +188,21 @@ Module BF.
       | bf_left bf' =>
         Some (bf_state bf' resets (pred ptr) tape input output)
       | bf_inc bf' =>
-        Some (bf_state bf' resets ptr (tape_inc tape ptr) input output)
+        Some (bf_state bf' resets ptr (BFTape.inc tape ptr) input output)
       | bf_dec bf' =>
-        Some (bf_state bf' resets ptr (tape_dec tape ptr) input output)
+        Some (bf_state bf' resets ptr (BFTape.dec tape ptr) input output)
       | bf_out bf' =>
-        Some (bf_state bf' resets ptr tape input (output ++ [tape_get tape ptr]))
+        Some (bf_state bf' resets ptr tape input
+                       (output ++ [BFTape.get tape ptr]))
       | bf_in bf' =>
         match input with
         | [] =>
-          Some (bf_state bf' resets ptr (tape_set tape ptr 0) input output)
+          Some (bf_state bf' resets ptr (BFTape.put tape ptr 0) input output)
         | x :: input' =>
-          Some (bf_state bf' resets ptr (tape_set tape ptr x) input' output)
+          Some (bf_state bf' resets ptr (BFTape.put tape ptr x) input' output)
         end
       | bf_loop inner_bf bf' =>
-        if Z.eqb (tape_get tape ptr) Z.zero then
+        if (BFTape.get tape ptr) =? 0 then
           Some (bf_state bf' resets ptr tape input output)
         else
           Some (bf_state inner_bf (bf :: resets) ptr tape input output)
@@ -224,7 +210,7 @@ Module BF.
     end.
 
   (* TODO: Use N as fuel with {measure N.to_nat fuel} *)
-  Function bf_run (state: BFState) (fuel: nat): option (list Z) :=
+  Function bf_run (state: BFState) (fuel: nat): option (list nat) :=
     match fuel with
     | 0 => None
     | S f =>
@@ -234,49 +220,37 @@ Module BF.
       end
     end.
 
-  Function z_of_ascii (a: ascii): Z :=
-    Z.of_nat (nat_of_ascii a).
-
-  Function ascii_of_z (z: Z): option ascii :=
-    match z with
-    | Zpos p => Some (ascii_of_pos p)
-    | _ => None
-    end.
-
   Function opt_list_len {A: Type} (l: option (list A)): nat :=
     match l with
     | Some l => List.length l
     | None => 0
     end.
 
-  Function string_of_zs (out: list Z): string :=
+  Function string_of_nats (out: list nat): string :=
     match out with
     | [] => EmptyString
-    | z :: zs' =>
-      match ascii_of_z z with
-      | None => EmptyString
-      | Some a => String a (string_of_zs zs')
-      end
+    | n :: ns' => String (ascii_of_nat n) (string_of_nats ns')
     end.
 
-  Function zs_of_string (str: string): list Z :=
+  Function nats_of_string (str: string): list nat :=
     match str with
     | EmptyString => []
-    | String a str' => z_of_ascii a :: (zs_of_string str')
+    | String a str' => nat_of_ascii a :: (nats_of_string str')
     end.
 
   (* The important interpreter as far as the spec is concerned *)
-  Function interpret_bf (prog: string) (zs: list Z) (f: nat): option (list Z) :=
+  Function interpret_bf (prog: string) (input: list nat) (f: nat):
+    option (list nat) :=
     match parse_bf prog with
     | None => None
-    | Some bf => bf_run (bf_state_init bf zs) f
+    | Some bf => bf_run (bf_state_init bf input) f
     end.
 
   Function interpret_bf_readable (prog: string) (input: string) (f:nat):
     string :=
-    match interpret_bf prog (zs_of_string input) f with
+    match interpret_bf prog (nats_of_string input) f with
     | None => EmptyString
-    | Some zs => string_of_zs zs
+    | Some output => string_of_nats output
     end.
 
   Example hello_world_bf:
