bftape.v
@@ -1,0 +1,27 @@
+Require FMapList.
+Require Import OrderedType OrderedTypeEx.
+
+Module BFTape.
+
+  (* A BFTape is a map from [nat] indices to [nat] values *)
+  Module NatMap := FMapList.Make Nat_as_OT.
+  Definition Tape := NatMap.t nat.
+
+  Definition empty := NatMap.empty nat.
+
+  Definition get (tape: Tape) (ptr: nat): nat :=
+    match (NatMap.find ptr tape) with
+    | Some x => x
+    | None => 0
+    end.
+
+  Definition put (tape: Tape) (ptr: nat) (x: nat): Tape :=
+    NatMap.add ptr x tape.
+
+  Definition inc (tape: Tape) (ptr: nat): Tape :=
+    put tape ptr (S (get tape ptr)).
+
+  Definition dec (tape: Tape) (ptr: nat): Tape :=
+    put tape ptr (pred (get tape ptr)).
+
+End BFTape.
